Lots of work with monadic_rewrite to show preemption_f is equivalent to a much simpler monad, if will_domain_switch holds
Signed-off-by: Scott Buckley <s.buckley@unsw.edu.au>

proof/infoflow/timeprotection/TimeProtectionIntegration.thy
@@ -10,9 +10,14 @@ imports TimeProtection
   "InfoFlow.Noninterference" schedule_oracle
 begin
 
-type_synonym if_other_state = "(user_context \<times> det_ext Structures_A.state) \<times> sys_mode"
+type_synonym context_and_state = "user_context \<times> det_ext Structures_A.state"
+type_synonym if_other_state    = "context_and_state \<times> sys_mode"
+
+(* domain-switch monad? *)
+
 
 locale integration_setup = 
+  Arch +
   time_protection_hardware
     gentypes
     PSched +
@@ -97,19 +102,9 @@ locale integration =
     "ii.part \<circ> fst" ma_uwr PSched "[]" "step_is_uwr_determined \<circ> fst" "step_is_publicly_determined \<circ> fst" select_trace 
   for gentypes :: "('fch \<times> 'fch_cachedness \<times> 'pch \<times> 'pch_cachedness \<times> 'l partition \<times> 'colour) itself"
   and select_trace and step_is_uwr_determined and step_is_publicly_determined
-  +
-  (*FIXME: getActiveIRQ is an Arch specific machine monad. I propose that we add this to the
-  arch interface, so we can reference it here. It would be a function that will return the
-  same result as getActiveIRQ, but does not increment the state. This function existing
-  assumes that getActiveIRQ always returns a single output state/value. *)
-  fixes peekActiveIRQ :: "bool \<Rightarrow> machine_state \<Rightarrow> irq option"
+  
 begin
 
-term getActiveIRQ
-
-lemma peekActiveIRQ_uwr:
-  "peekActiveIRQ False (machine_state s) = peekActiveIRQ False (machine_state t)"
-oops
 (* what do we know
   we definitely have interrupted_modes of os.
   but that incluedes both
@@ -121,18 +116,18 @@ oops
 
 *)
 
-(* check_active_irq_A_if *)
+definition is_timer_irq :: "det_ext Structures_A.state \<Rightarrow> bool" where
+  "is_timer_irq s \<equiv> let irq = irq_oracle (Suc (irq_state_of_state s)) in
+                     \<exists>s'. (Some irq, s') \<in> fst (do_machine_op (getActiveIRQ False) s)
+                           \<and> interrupt_states s irq = IRQTimer"
 
-(* definition IsActiveIrq *)
+definition domain_time_zero :: "if_other_state \<Rightarrow> bool" where
+  "domain_time_zero os \<equiv> domain_time_internal (exst (snd (fst os))) = 1"
 
 definition will_domain_switch :: "if_other_state \<Rightarrow> bool" where
-  "will_domain_switch os \<equiv> case snd os of
-    KernelEntry Interrupt \<Rightarrow> (
-      \<exists>irq s'. (fst os, Some irq, s') \<in> check_active_irq_A_if \<and>
-        (case interrupt_states (snd (fst os)) irq of
-         IRQTimer \<Rightarrow> domain_time_internal (exst (snd (fst os))) = 1
-       | _ \<Rightarrow> False))
-  | _ \<Rightarrow> False"
+  "will_domain_switch os \<equiv> interrupted_modes (snd os)
+                         \<and> is_timer_irq (snd (fst os))
+                         \<and> domain_time_zero os"
 
 lemma ex_eq:
   "(\<exists>y. (P y = P' y)) \<Longrightarrow>(\<exists>x. P x) = (\<exists>x. P' x)"
@@ -141,14 +136,716 @@ lemma ex_eq:
 lemma will_domain_switch_from_uwr:
   "uwr2 os PSched ot \<Longrightarrow>
   will_domain_switch ot = will_domain_switch os"
+  unfolding uwr_def
   apply (clarsimp simp: will_domain_switch_def uwr_def sameFor_def sameFor_scheduler_def)
   apply (case_tac bc; case_tac ba; clarsimp split:event.splits)
     
     apply (prop_tac "interrupt_states (internal_state_if ((aa, bb), KernelEntry Interrupt))
                    = interrupt_states (internal_state_if ((a , b ), KernelEntry Interrupt))")
      apply simp 
-     
+     subgoal sorry
+  oops
+
+definition can_split_four_ways where
+  "can_split_four_ways s1 s5 oldclean dirty gadget newclean \<equiv>
+   \<exists> s2 s3 s4. s2 \<in> oldclean s1 \<and> s3 \<in> dirty s2 \<and> s4 \<in> gadget s3 \<and> s4 \<in> newclean s4"
+
+lemma step_bigstepR:
+  "(s, s') \<in> Step () \<Longrightarrow>
+  big_step_R s s'"
+  apply (drule big_Step2, rule small_step_to_big_step; simp)
+  done
+
+term global_automaton_if
+term ADT_A_if
+
+find_theorems name:obs_det
+
+lemma big_step_Init:
+  "(s1, s3) \<in> Step () \<Longrightarrow>
+  Init (ADT_A_if utf) s1 = {s1}"
+  apply (clarsimp simp:system.Step_def execution_def big_step_ADT_A_if_def
+    big_step_adt_def Fin_ADT_if)
+  apply (prop_tac "s1 \<in> full_invs_if")
+   apply (smt (verit, best) ImageE Init_ADT_if IntE empty_iff foldl.simps(1)
+     foldl.simps(2) insert_iff steps_def)
+  apply (prop_tac "step_restrict s1")
+   apply (metis (no_types, lifting) ADT_A_if_def IntE Step_big_step_ADT_A_if big_step_ADT_A_if_def
+     big_step_adt_def data_type.simps(1) mem_Collect_eq singletonD steps_eq_Run)
+  apply (clarsimp simp: Init_ADT_if)
+  done
+
+
+inductive_set sub_big_steps_alt
+  :: "('istate,'estate,'event) data_type \<Rightarrow> ('istate \<Rightarrow> bool) \<Rightarrow> ('istate \<times> 'istate \<times> 'event list) set"
+  for A :: "('istate,'estate,'event) data_type" and J :: "('istate \<Rightarrow> bool)"
+where
+  nil: "\<lbrakk>evlist = []; s2 = s1; \<not> J s1\<rbrakk> \<Longrightarrow>  (s1, s2, evlist) \<in> sub_big_steps_alt A J" |
+  step: "\<lbrakk>evlist = [e] @ evlist'; (s2, s3, evlist') \<in> sub_big_steps_alt A J;
+          (s1, s2) \<in> data_type.Step A e; \<not> J s2\<rbrakk> \<Longrightarrow> (s1, s3, evlist) \<in> sub_big_steps_alt A J"
+                                          
+
+
+lemma sub_big_steps_sub_big_steps_alt_aux:
+ " (s2, es1) \<in> sub_big_steps A R s1 \<Longrightarrow>    
+   (s2, s3, es2) \<in> sub_big_steps_alt A (\<lambda> b. R s1 b) \<Longrightarrow>
+   (s1, s3, es1 @ es2) \<in> sub_big_steps_alt A (\<lambda> b. R s1 b)"
+  apply (induct s2 es1 arbitrary:s3 es2 rule:sub_big_steps.induct)
+   apply clarsimp
+  apply clarsimp
+  apply (simp add: sub_big_steps_alt.step)
+  done
+
+
+
+lemma sub_big_steps_sub_big_steps_alt:
+ "(s2, es1) \<in> sub_big_steps A R s1 \<Longrightarrow>    
+  (s1, s2, es1) \<in> sub_big_steps_alt A (\<lambda> b. R s1 b)"
+  by (metis (mono_tags) append_Nil2 sub_big_steps_Run sub_big_steps_alt.nil sub_big_steps_sub_big_steps_alt_aux)
+
+(*
+lemma big_stepsD:
+  "(s,t) \<in> big_steps A R exmap ev
+   \<Longrightarrow> \<exists>s' as a. (s',as) \<in> sub_big_steps A R s \<and> (s',t) \<in> Step A a \<and> R s t \<and> ev = exmap (as @ [a])"
+  apply (erule big_steps.induct)
+  apply blast
+  done
+*)
+
+term global_automaton_if
+
+lemma step_to_KernelExit:
+  "(s1, s2) \<in> data_type.Step (ADT_A_if utf) () \<Longrightarrow>
+  snd s2 = KernelExit \<Longrightarrow>
+  \<exists>b. snd s1 = KernelSchedule b"
+  apply (cases s2, clarsimp)
+  apply (clarsimp simp: ADT_A_if_def global_automaton_if_def)
+  apply (erule disjE; clarsimp)
+  apply (clarsimp simp: kernel_exit_A_if_def split:if_splits)
+  done
+
+lemma schedule_step':
+  assumes schedule:
+    "\<And>r. \<lbrakk> (r,internal_state_if s') \<in> fst (schedule_if (user_context_of s) (internal_state_if s));
+            sys_mode_of s' = KernelExit; r = user_context_of s; r = user_context_of s' \<rbrakk>
+            \<Longrightarrow> P"
+  shows
+    "\<lbrakk> (sys_mode_of s') = KernelExit; (s,s') \<in> data_type.Step (ADT_A_if utf) () \<rbrakk>
+       \<Longrightarrow> P"
+  apply (frule step_to_KernelExit, simp add: sys_mode_of_def)
+  apply (insert schedule)
+  apply (metis schedule_step sys_mode_of_def)
+  done
+
+lemma step_to_KernelSchedule:
+  "(s1, s2) \<in> data_type.Step (ADT_A_if utf) () \<Longrightarrow>
+  snd s2 = KernelSchedule True \<Longrightarrow>
+  interrupted_modes (snd s1)"
+  apply (cases s2, clarsimp)
+  apply (clarsimp simp: ADT_A_if_def global_automaton_if_def)
+  apply (elim disjE; clarsimp)
+   apply (clarsimp simp: kernel_exit_A_if_def split:if_splits)
+  done
+
+lemma interrupt_step':
+  assumes interrupt:
+    "\<And>r. (r,internal_state_if s')
+            \<in> fst (kernel_entry_if Interrupt (user_context_of s) (internal_state_if s))
+          \<Longrightarrow> sys_mode_of s = KernelEntry Interrupt \<Longrightarrow> (sys_mode_of s' = KernelSchedule True)
+          \<Longrightarrow> snd r = user_context_of s \<Longrightarrow> snd r = user_context_of s'
+          \<Longrightarrow> cur_domain (internal_state_if s') = cur_domain (internal_state_if s)
+          \<Longrightarrow> P"
+  assumes preemption:
+    "\<And>r. (r,internal_state_if s')
+            \<in> fst (handle_preemption_if (user_context_of s) (internal_state_if s))
+          \<Longrightarrow> sys_mode_of s = KernelPreempted \<Longrightarrow> sys_mode_of s' = KernelSchedule True
+          \<Longrightarrow> r = user_context_of s \<Longrightarrow> r = user_context_of s'
+          \<Longrightarrow> cur_domain (internal_state_if s') = cur_domain (internal_state_if s)
+          \<Longrightarrow> P"
+  shows "\<lbrakk> interrupted_modes (sys_mode_of s); (s,s') \<in> data_type.Step (ADT_A_if utf) () \<rbrakk> \<Longrightarrow> P"
+  apply (insert interrupt preemption)
+  oops
+
+lemma interrupted_modes_PSched:
+ "interrupted_modes (snd s1) \<Longrightarrow>
+  part s1 = PSched"
+  apply (cases s1; clarsimp)
+  apply (case_tac ba; clarsimp simp:part_def)
+  done
+
+lemma kernel_entry_if_Inr:
+  "\<lbrace>\<top>\<rbrace> kernel_entry_if Interrupt ab \<lbrace>\<lambda>r s. fst r=Inr ()\<rbrace>"
+  apply (wpsimp simp: kernel_entry_if_def liftE_def)
+  done
+
+lemma domainswitch_two_paths:
+  "(s1, s3) \<in> Step () \<Longrightarrow>
+  interrupted_modes (snd s1) \<Longrightarrow>
+  \<exists>s2. (s2, (), fst s3) \<in> kernel_schedule_if \<and>
+       ((fst s1, (), s2) \<in> kernel_handle_preemption_if
+      \<or> (fst s1, False, s2) \<in> kernel_call_A_if Interrupt)"
+  apply (drule big_Step2)
+  apply (rule_tac s=s1 and s''=s3 in scheduler_steps)
+    apply assumption
+   apply (rule interrupted_modes_PSched; simp)
+  apply (rename_tac s2, thin_tac "(s1, s3) \<in> _")
+  apply (rule_tac x="fst s2" in exI)
+  apply (intro conjI)
+
+   \<comment> \<open>the second step (schedule)\<close>
+   apply (rule schedule_step; simp)
+   apply (clarsimp simp: kernel_schedule_if_def user_context_of_def)
+
+  apply (rule_tac s=s1 and s'=s2 in interrupt_step; simp add:sys_mode_of_def)
+   \<comment> \<open>the first step (kernel call, interrupt)\<close>
+   apply (intro disjI2)
+   apply (cases s1; clarsimp)
+   apply (clarsimp simp: kernel_call_A_if_def)
+   apply (rule_tac x=False in exI; simp)
+   using use_valid kernel_entry_if_Inr apply fastforce
+
+  \<comment> \<open>the first step (kernel preempted)\<close>
+  apply (intro disjI1)
+  apply (cases s1; clarsimp)
+  apply (clarsimp simp: kernel_handle_preemption_if_def)
+  done
+
+lemma kernel_handle_preemption_if_handle_preemption_if:
+  "((fst s1, (), s2) \<in> kernel_handle_preemption_if)
+  = (s2 \<in> fst (handle_preemption_if (fst (fst s1)) (snd (fst s1))))"
+  apply (clarsimp simp:kernel_handle_preemption_if_def split:prod.splits)
+  done
+
+crunches arch_mask_irq_signal
+  for scheduler_action: "\<lambda>s. P (scheduler_action s)"
+
+definition
+  handle_interrupt_IRQTimer where
+ "handle_interrupt_IRQTimer \<equiv>
+   do
+     modify (\<lambda>s. s\<lparr>machine_state :=
+       machine_state s \<lparr>irq_state := irq_state_of_state s + 1\<rparr>\<rparr>);
+     do_extended_op timer_tick;
+     do_machine_op resetTimer
+   od"
+
+lemma weirdthing:
+  "\<lbrakk>A; B\<rbrakk> \<Longrightarrow> A \<and> B"
+  by simp
+
+find_theorems getActiveIRQ name:wp
+
+thm dmo_getActiveIRQ_wp
+
+find_theorems name:gets
+
+definition irq_at' :: "nat \<Rightarrow> irq option" where
+  "irq_at' pos \<equiv> Some (irq_oracle pos)"
+
+definition Psame :: "'a \<Rightarrow> 'b \<Rightarrow> 'a \<Rightarrow> 'b \<Rightarrow> bool" where
+  "Psame a b = (\<lambda>a' b'. a'=a \<and> b'=b)"
+
+lemma dmo_getActiveIRQ_timer:
+  "\<lbrace>\<lambda>s. is_timer_irq s \<and> P (Some (irq_oracle (irq_state (machine_state s)+1)))
+  (s\<lparr>machine_state := (machine_state s\<lparr>irq_state := irq_state (machine_state s) + 1\<rparr>)\<rparr>)\<rbrace>
+     do_machine_op (getActiveIRQ True)
+   \<lbrace>\<lambda>r s. P r s \<and> interrupt_states s (the r) = IRQTimer\<rbrace>"
+  apply (clarsimp simp: getActiveIRQ_no_non_kernel_IRQs)
+  apply (rule hoare_weaken_pre)
+  apply (rule dmo_getActiveIRQ_wp)
+  apply (clarsimp simp: is_timer_irq_def check_active_irq_A_if_def check_active_irq_if_def)
+  apply (clarsimp simp: bind_def do_machine_op_def return_def)
+  apply (clarsimp simp: gets_def bind_def return_def)
+  apply (clarsimp simp: modify_def bind_def get_def put_def select_f_def)
+  apply (clarsimp simp: getActiveIRQ_def bind_def gets_def get_def return_def modify_def put_def)
+  apply (clarsimp simp:irq_at_def Let_def)
+  apply (clarsimp split:if_splits)
+   apply (simp add: in_monad(12))
+  (* apply (clarsimp simp:return_def) *)
+  done
   
+lemma dmo_getActiveIRQ_timer_withoutextras:
+  "\<lbrace>\<lambda>s. is_timer_irq s \<and> P (Some (irq_oracle (irq_state (machine_state s)+1)))
+  (s\<lparr>machine_state := (machine_state s\<lparr>irq_state := irq_state (machine_state s) + 1\<rparr>)\<rparr>)\<rbrace>
+     do_machine_op (getActiveIRQ True)
+   \<lbrace>P\<rbrace>"
+  apply (rule hoare_strengthen_post)
+  apply (rule dmo_getActiveIRQ_timer)
+  apply simp
+  done
+
+
+lemma dmo_getActiveIRQ_timer2:
+  "\<lbrace>\<lambda>s. is_timer_irq s\<rbrace>
+     do_machine_op (getActiveIRQ True)
+   \<lbrace>\<lambda>r s. r = Some (irq_oracle (irq_state (machine_state s)))
+      \<and> interrupt_states s (the r) = IRQTimer\<rbrace>"
+  apply (clarsimp simp: getActiveIRQ_no_non_kernel_IRQs)
+  apply (rule hoare_weaken_pre)
+  apply (rule dmo_getActiveIRQ_wp)
+  apply (clarsimp simp: is_timer_irq_def check_active_irq_A_if_def check_active_irq_if_def)
+  apply (clarsimp simp: bind_def do_machine_op_def return_def)
+  apply (clarsimp simp: gets_def bind_def return_def)
+  apply (clarsimp simp: modify_def bind_def get_def put_def select_f_def)
+  apply (clarsimp simp: getActiveIRQ_def bind_def gets_def get_def return_def modify_def put_def)
+  apply (clarsimp simp:irq_at_def Let_def)
+  apply (clarsimp split:if_splits)
+   apply (simp add: in_monad(12))
+  (* apply (clarsimp simp:return_def) *)
+  done
+
+find_theorems monadic_rewrite name:"wp"
+
+find_theorems getActiveIRQ valid
+
+thm dmo_getActiveIRQ_wp
+
+
+
+term "do_machine_op (getActiveIRQ True)"
+
+(*
+lemma dmo_getActiveIRQ_wp[CNode_IF_assms]:
+  "\<lbrace>\<lambda>s. is_timer_irq s \<and> (P (irq_at' (irq_state (machine_state s) + 1))
+          (s\<lparr>machine_state := (machine_state s\<lparr>irq_state := irq_state (machine_state s) + 1\<rparr>)\<rparr>))\<rbrace>
+   do_machine_op (getActiveIRQ b) :: user_context \<times> det_ext Structures_A.state
+   \<lbrace>P\<rbrace>"
+  apply (simp add: do_machine_op_def getActiveIRQ_def non_kernel_IRQs_def)
+  apply (wp modify_wp | wpc)+
+  apply clarsimp
+  apply (erule use_valid)
+   apply (wp modify_wp)
+  apply (auto simp: irq_at_def Let_def split: if_splits)
+  done
+*)
+
+lemma set_ext:
+  "(\<forall>x. (x \<in> S) = (x \<in> T)) \<Longrightarrow> (S = T)"
+  apply blast
+  done
+
+lemma pair_eq:
+  "(fst f = fst g) \<Longrightarrow> snd f = snd g \<Longrightarrow> (f = g)"
+  by (simp add: prod.expand)
+
+lemma ex_eq:
+  "P = Q \<Longrightarrow> ((\<exists>x. P) = (\<exists>x. Q))"
+  by simp
+
+
+lemma det_empty_fail:
+  "det f \<Longrightarrow> empty_fail f"
+  apply (clarsimp simp:empty_fail_def det_def)
+  by (metis insert_not_empty prod.sel(1))
+
+lemma det_no_fail:
+  "det f \<Longrightarrow> no_fail \<top> f"
+  apply (clarsimp simp:no_fail_def det_def)
+  by (metis prod.sel(2))
+
+lemma weak_pre_to_strong_post:
+  "\<forall>P. \<lbrace>\<lambda>s. P (Pr s) (Ps s)\<rbrace> f \<lbrace>P\<rbrace> \<Longrightarrow>
+  \<forall>s. \<lbrace>\<lambda>s'. s'=s\<rbrace> f \<lbrace>\<lambda>r' s'. r'=Pr s \<and> s'=Ps s\<rbrace>"
+  by (smt (verit, best) hoare_strengthen_pre_via_assert_forward)
+
+lemma strong_post_elim:
+  "empty_fail f \<Longrightarrow>
+   no_fail \<top> f \<Longrightarrow>
+    (\<forall>s. \<lbrace>\<lambda>s'. s'=s\<rbrace> f \<lbrace>\<lambda>r' s'. r'=Pr s \<and> s'=Ps s\<rbrace>) \<Longrightarrow>
+    f = 
+    (do s \<leftarrow> get; modify Ps; return (Pr s) od)"
+  apply (rule ext)
+  apply (clarsimp simp: valid_def)
+  apply (drule_tac x=x in spec)
+  apply (clarsimp simp:exec_get exec_modify)
+  apply (clarsimp simp:return_def)
+  apply (rule pair_eq; clarsimp)
+   apply (rule set_ext; clarsimp)
+   apply (case_tac "((a, b) \<in> fst (f x))"; clarsimp)
+    apply (drule_tac x="(a, b)" in bspec, assumption)
+    apply clarsimp
+   apply (clarsimp simp: empty_fail_def no_fail_def)
+   apply fastforce
+  apply (clarsimp simp:no_fail_def)
+  done
+
+lemma weak_pre_elim:
+  "empty_fail f \<Longrightarrow>
+   no_fail \<top> f \<Longrightarrow>
+    (\<forall>P. \<lbrace>\<lambda>s. P (Pr s) (Ps s)\<rbrace> f \<lbrace>P\<rbrace>) \<Longrightarrow>
+    f = 
+    (do s \<leftarrow> get; modify Ps; return (Pr s) od)"
+  apply (drule weak_pre_to_strong_post)
+  apply (erule strong_post_elim; simp)
+  done
+
+lemma weak_pre_elim_P:
+  "empty_fail f \<Longrightarrow>
+   no_fail \<top> f \<Longrightarrow>
+    (\<forall>P. \<lbrace>\<lambda>s.(P' s \<and>  P (Pr s) (Ps s))\<rbrace> f \<lbrace>P\<rbrace>) \<Longrightarrow>
+    P' s' \<Longrightarrow>
+    f s' = 
+    (do s \<leftarrow> get; modify Ps; return (Pr s) od) s'"
+  apply (clarsimp simp: valid_def)
+  apply (clarsimp simp:exec_get exec_modify)
+  apply (clarsimp simp:return_def)
+  apply (drule_tac x="\<lambda>r s. r=Pr s' \<and> s=Ps s'" in spec)
+  apply (drule_tac x=s' in spec)
+  apply (rule pair_eq; clarsimp)
+   apply (rule set_ext; clarsimp)
+   apply (case_tac "((a, b) \<in> fst (f s'))"; clarsimp)
+    apply (drule_tac x="(a, b)" in bspec, assumption)
+    apply clarsimp
+   apply (clarsimp simp: empty_fail_def no_fail_def)
+   apply fastforce
+  apply (clarsimp simp:no_fail_def)
+  done
+
+lemma weak_pre_rewrite_P:
+  "empty_fail f \<Longrightarrow>
+   no_fail \<top> f \<Longrightarrow>
+    (\<forall>P. \<lbrace>\<lambda>s.(P' s \<and>  P (Pr s) (Ps s))\<rbrace> f \<lbrace>P\<rbrace>) \<Longrightarrow>
+    monadic_rewrite E F
+      P'
+      f
+      (do z \<leftarrow> get; modify Ps; return (Pr z) od)"
+  apply (clarsimp simp: monadic_rewrite_def)
+  apply (drule(3) weak_pre_elim_P)
+  apply simp
+  done
+
+lemma rewrite_return_bind:
+  "monadic_rewrite E F
+      P
+      (do z \<leftarrow> f1; f2 z; return (f3 z) od >>= g)
+      (do z \<leftarrow> f1; f2 z; g (f3 z) od)"
+  apply (clarsimp simp: monadic_rewrite_def)
+  apply (smt (verit, ccfv_SIG) NonDetMonad.bind_assoc arg_cong_bind1
+    let_into_return set_eq_subset)
+  done
+
+lemma weak_pre_rewrite_bind_aux:
+  "empty_fail f \<Longrightarrow>
+   no_fail \<top> f \<Longrightarrow>
+    (\<forall>P. \<lbrace>\<lambda>s.(P' s \<and>  P (Pr s) (Ps s))\<rbrace> f \<lbrace>P\<rbrace>) \<Longrightarrow>
+    monadic_rewrite E F
+      P'
+      (f >>= g)
+      (do z \<leftarrow> get; modify Ps; return (Pr z) od >>= g)"
+  apply (rule monadic_rewrite_bind_head)
+  apply (rule weak_pre_rewrite_P; simp)
+  done
+
+lemma weak_pre_rewrite_bind:
+  "empty_fail f \<Longrightarrow>
+   no_fail \<top> f \<Longrightarrow>
+    (\<forall>P. \<lbrace>\<lambda>s.(P' s \<and>  P (Pr s) (Ps s))\<rbrace> f \<lbrace>P\<rbrace>) \<Longrightarrow>
+    monadic_rewrite E F
+      P'
+      (f >>= g)
+      (do z \<leftarrow> get; modify Ps; g (Pr z) od)"
+  apply (rule monadic_rewrite_imp)
+  apply (rule monadic_rewrite_trans)
+  apply (rule weak_pre_rewrite_bind_aux, assumption+)
+  apply (rule rewrite_return_bind)
+  apply simp
+  done
+
+
+(* not needed i guess. they're true though
+lemma and_refl [simp]:
+  "(P and P) = P"
+  by (simp add: pred_conj_def)
+
+lemma no_fail_bind_simple:
+  assumes f: "no_fail P f"
+  assumes g: "\<And>rv. no_fail (R rv) (g rv)"
+  assumes v: "\<lbrace>P\<rbrace> f \<lbrace>R\<rbrace>"
+  shows "no_fail P (f >>= (\<lambda>rv. g rv))"
+  apply (insert f g v)
+  apply (rule no_fail_bind [where P=P and Q=P and R=R, simplified]; assumption)
+  done
+
+lemma no_fail_bind_simple_top:
+  assumes f: "no_fail P f"
+  assumes g: "\<And>rv. no_fail \<top> (g rv)"
+  shows "no_fail P (f >>= (\<lambda>rv. g rv))"
+  apply (insert f g)
+  apply (rule no_fail_bind [where Q=\<top>, simplified])
+    apply assumption
+   apply assumption
+  apply (clarsimp simp:valid_def)
+  done
+*)
+
+lemma do_machine_op_no_fail [wp_unsafe]:
+  "no_fail Q f \<Longrightarrow>
+  (\<forall>s. P s \<longrightarrow> Q (machine_state s)) \<Longrightarrow>
+  no_fail P (do_machine_op f)"
+  apply (clarsimp simp:do_machine_op_def)
+  apply wpsimp
+  apply (clarsimp simp: no_fail_def)
+  done
+
+lemma dmo_getActiveIRQ_no_fail:
+  "no_fail \<top> (do_machine_op (getActiveIRQ True))"
+  apply (wpsimp wp:do_machine_op_no_fail)
+  done
+
+lemma monadic_rewrite_dmo_getActiveIRQ:
+  "monadic_rewrite E F
+    is_timer_irq
+    (do_machine_op (getActiveIRQ True))
+    (do s \<leftarrow> get;
+       modify (\<lambda>s. s\<lparr>machine_state := machine_state s\<lparr>irq_state := irq_state_of_state s + 1\<rparr>\<rparr>);
+       return (Some (irq_oracle (irq_state_of_state s + 1))) od)"
+  apply (rule weak_pre_rewrite_P)
+    apply (rule do_machine_op_empty_fail, rule getActiveIRQ_empty_fail)
+   apply (rule dmo_getActiveIRQ_no_fail)
+  using dmo_getActiveIRQ_timer_withoutextras apply clarsimp
+  done
+
+lemma monadic_rewrite_dmo_getActiveIRQ_bind:
+  "monadic_rewrite E F
+    is_timer_irq
+    (do_machine_op (getActiveIRQ True) >>= g)
+    (do s \<leftarrow> get;
+       modify (\<lambda>s. s\<lparr>machine_state := machine_state s\<lparr>irq_state := irq_state_of_state s + 1\<rparr>\<rparr>);
+       g (Some (irq_oracle (irq_state_of_state s + 1))) od)"
+  apply (rule weak_pre_rewrite_bind)
+    apply (rule do_machine_op_empty_fail, rule getActiveIRQ_empty_fail)
+   apply (rule dmo_getActiveIRQ_no_fail)
+  using dmo_getActiveIRQ_timer_withoutextras apply clarsimp
+  done
+
+lemma pred_conj_refl:
+  "(P and P) = P"
+  by (simp add: pred_conj_def)
+
+
+lemma bind_assoc_sym:
+  "do a \<leftarrow> f; b \<leftarrow> g a; h b od = 
+  (do a \<leftarrow> f; g a od) >>= h"
+  by (simp add: bind_subst_lift)
+
+lemma get_modify_use_reorder:
+  "(\<forall>s. Pr' (Ps s) = Pr s) \<Longrightarrow>
+  (do z <- get;
+     y \<leftarrow> modify Ps;
+     handle_interrupt (Pr z)
+   od) = 
+  (do y \<leftarrow> modify Ps;
+     z <- get;
+     handle_interrupt (Pr' z)
+   od)"
+  apply (rule ext)
+  apply (clarsimp simp: exec_get exec_modify)
+  done
+
+lemma monadic_rewrite_remove_get:
+  "monadic_rewrite E F
+    P
+    (do s \<leftarrow> get; f od)
+    f"
+  by (simp add: exec_get monadic_rewrite_refl3)
+
+lemma monadic_rewrite_remove_used_get:
+  "(\<forall>s. Ps \<longrightarrow> Q (e s)) \<Longrightarrow>
+  Q r \<Longrightarrow>
+  monadic_rewrite E F
+    P
+    f
+    (g r) \<Longrightarrow>
+  monadic_rewrite E F
+    P
+    f
+    (do s \<leftarrow> get; g (e s) od)"
+  oops
+
+lemma sdsdfsdfdd:
+  "(do s \<leftarrow> get; f s od) =
+    (\<lambda>s. f s s)"
+  by (simp add: exec_get monadic_rewrite_refl3 monadic_rewrite_to_eq)
+
+lemma monadic_rewrite_double_get:
+  "monadic_rewrite E F P (do s \<leftarrow> get; s' \<leftarrow> get; m s s' od) (do s \<leftarrow> get; m s s od)"
+  by (simp add: exec_get monadic_rewrite_refl3)
+
+lemma monadic_rewrite_trans_simple:
+  "\<lbrakk> monadic_rewrite F E P f g; monadic_rewrite F E P g h \<rbrakk>
+      \<Longrightarrow> monadic_rewrite F E P f h"
+  by (auto simp add: monadic_rewrite_def)
+
+thm monadic_rewrite_bind_tail
+lemma monadic_rewrite_bind_tail_result:
+  "\<lbrakk>(\<And>x. Q x \<longrightarrow> monadic_rewrite F E P (h x) (j x)); \<lbrace>R\<rbrace> f \<lbrace>\<lambda>r s. Q r \<and> P s\<rbrace>\<rbrakk> \<Longrightarrow>
+  monadic_rewrite F E R (f >>= h) (f >>= j)"
+  by (smt (z3) monadic_rewrite_bind_tail monadic_rewrite_imp monadic_rewrite_refl3)
+
+lemma monadic_rewrite_bind_get:
+  "\<lbrakk>(\<And>x. P x \<longrightarrow> monadic_rewrite F E P (h x) (j x))\<rbrakk> \<Longrightarrow>
+  monadic_rewrite F E P (get >>= h) (get >>= j)"
+  apply (erule monadic_rewrite_bind_tail_result)
+  apply (clarsimp simp:valid_def get_def)
+  done
+
+thm monadic_rewrite_name_pre
+
+thm monadic_rewrite_refl
+lemma monadic_rewrite_refl2:
+  "monadic_rewrite F E P f f"
+  by (simp add: monadic_rewrite_def)
+
+lemma sdsdf:
+  "monadic_rewrite E F
+    is_timer_irq
+    (handle_preemption_if tc)
+    (do handle_interrupt_IRQTimer; return tc od)"
+  apply (clarsimp simp: handle_preemption_if_def)
+  (* get rid of the "return tc" at the end *)
+  apply (subst bind_assoc_sym)
+  apply (rule monadic_rewrite_bind_head)
+
+  apply (rule monadic_rewrite_trans_simple)
+   apply (rule monadic_rewrite_dmo_getActiveIRQ_bind)
+  apply clarsimp
+
+  apply (subst get_modify_use_reorder [where Pr'="\<lambda>s. irq_oracle (irq_state_of_state s)"])
+   apply clarsimp
+
+  apply (clarsimp simp: handle_interrupt_IRQTimer_def)
+  
+  apply (rule monadic_rewrite_bind_tail [
+    where Q="\<lambda>r s. interrupt_states s (irq_oracle (irq_state_of_state s)) = IRQTimer"])
+   defer
+   apply (clarsimp simp: valid_def is_timer_irq_def Let_def)
+   apply (clarsimp simp: simpler_modify_def)  
+  apply clarsimp
+  
+  (*
+  apply (rule monadic_rewrite_imp)
+  apply (rule monadic_rewrite_trans)
+  apply (rule monadic_rewrite_remove_used_get [where g=handle_interrupt])
+  *)
+
+
+  find_theorems monadic_rewrite If
+
+  apply (clarsimp simp: handle_interrupt_def)
+  apply (prop_tac "\<forall>z. maxIRQ < irq_oracle (irq_state_of_state z) = False")
+   using irq_oracle_max_irq word_not_le apply blast
+  apply clarsimp
+  apply (thin_tac _)
+
+
+  apply (clarsimp simp: get_irq_state_def gets_def)
+
+  (* turn the two "get"s into one *)
+  apply (rule monadic_rewrite_trans_simple)
+  apply (rule monadic_rewrite_double_get)
+
+  apply (rule monadic_rewrite_trans_simple)
+   apply (rule monadic_rewrite_bind_get)
+   apply clarsimp
+   apply (rule monadic_rewrite_refl2)
+  apply (clarsimp simp:ackInterrupt_def)
+
+  find_theorems monadic_rewrite name:gen_asm
+
+  apply (rule monadic_rewrite_trans_simple)
+   apply (rule monadic_rewrite_remove_get)
+  apply (rule monadic_rewrite_refl2)
+  done
+  
+  
+  
+  
+
+
+
+lemma handle_interrupt_for_IRQTimer_aux:
+  "is_timer_irq (tc, s) \<Longrightarrow>
+  handle_preemption_if tc s = (do handle_interrupt_IRQTimer; return tc od) s"
+  apply (clarsimp simp: handle_preemption_if_def)
+  apply (clarsimp simp: getActiveIRQ_def do_machine_op_def)
+  oops
+
+lemma handle_interrupt_for_IRQTimer:
+  "\<lbrace>\<lambda>s. is_timer_irq (tc, s)\<rbrace> do handle_interrupt_IRQTimer; return tc od \<lbrace>Q\<rbrace> \<Longrightarrow>
+  \<lbrace>\<lambda>s. is_timer_irq (tc, s)\<rbrace> handle_preemption_if tc \<lbrace>Q\<rbrace>"
+  apply (wpsimp simp: handle_preemption_if_def)
+    prefer 2
+    apply (rule hoare_strengthen_post, rule dmo_getActiveIRQ_timer)
+    apply clarsimp
+
+  apply (clarsimp simp:valid_def)
+  apply (drule_tac x=s in spec)
+  using handle_interrupt_for_IRQTimer_aux apply fastforce
+  done
+
+lemma
+  "\<lbrace>\<lambda>s. is_timer_irq (tc, s)\<rbrace>
+    handle_preemption_if tc
+  \<lbrace>\<lambda>r s. scheduler_action s = choose_new_thread\<rbrace>"
+  apply (rule handle_interrupt_for_IRQTimer)
+  apply (wpsimp simp: handle_interrupt_IRQTimer_def)
+  (* more work to do here *)
+  
+  
+
+lemma first_bit_whatever_meow:
+  "(fst s1, (), s2) \<in> kernel_handle_preemption_if
+ \<or> (fst s1, False, s2) \<in> kernel_call_A_if Interrupt \<Longrightarrow>
+  scheduler_action (snd s2) = choose_new_thread"
+  apply (elim disjE)
+  apply (clarsimp simp: kernel_handle_preemption_if_handle_preemption_if)
+  apply (cases s1; clarsimp)
+
+lemma more_splits_test:
+  "(s1, (), s3) \<in> kernel_schedule_if \<Longrightarrow>
+   s1 = s3"
+  apply (cases s1)
+  pply (clarsimp simp: kernel_schedule_if_def schedule_if_def)
+
+
+lemma domainswitch_splits_four_ways:
+  "(s1, s5) \<in> Step () \<Longrightarrow>
+  will_domain_switch s1 \<Longrightarrow>
+  can_split_four_ways s1 s5 a b c d"
+  apply (frule step_bigstepR)
+  apply (clarsimp simp: big_step_R_def)
+  apply (erule disjE)
+   apply (clarsimp simp:will_domain_switch_def)
+  apply clarsimp
+
+  apply (drule(1) domainswitch_two_paths, clarsimp)
+  apply (rename_tac s2a s2b)
+  apply (simp add: kernel_handle_preemption_if_handle_preemption_if)
+
+  (* 
+     From big_step_R, we know that each step is either some user sequence,
+     or we are starting from the scheduler modes:
+     - KernelEntry Interrupt, or
+     - KernelPreempted
+
+     For each of these options, there are exactly TWO small steps that make up the big step,
+     and the second is identical. In the first step we take either:
+     - kernel_callf Interrupt
+     - preemptionf
+     ... and then we always perform `schedulef`.
+
+     We should make some lemmas that break this down for us so we can reason about those
+     individual steps.
+
+     I am still kinda trying to figure out if preemption can ever cause a (domain) schedule switch,
+     and if not, how do I prove this?
+ *)
+  apply (clarsimp simp:interrupted_modes_def)
+
+  apply (clarsimp simp: Step_def big_step_ADT_A_if_def)
+
+  apply (clarsimp simp:Step_def big_step_ADT_A_if_def system.Step_def big_step_adt_def
+    )
 
 interpretation ma?:time_protection_system PSched fch_lookup fch_read_impact fch_write_impact
   empty_fch fch_flush_cycles fch_flush_WCET pch_lookup pch_read_impact pch_write_impact do_pch_flush
@@ -157,12 +854,19 @@ interpretation ma?:time_protection_system PSched fch_lookup fch_read_impact fch_
   "big_step_ADT_A_if utf" s0 "policyFlows (pasPolicy initial_aag)" _ _ _ will_domain_switch
   
   apply unfold_locales
+               (* external_uwr_same_domain *)
                using schedIncludesCurrentDom apply presburger
+              (* external_uwr_equiv *)
               apply (simp add: uwr_equiv_rel)
+             (* will_domain_switch_public *)
              subgoal sorry
+            (* next_latest_domainswitch_in_future *)
             apply (rule nlds_in_future)
+           (* next_latest_domainswitch_flatsteps *)
            apply (rule nlds_flatsteps; simp)
+          (* get_next_domain_public *)
           subgoal sorry
+          (* get_domainswitch_middle_state_nonempty *)
          subgoal sorry
         subgoal sorry
        subgoal sorry
